wasm-proofs/Wasm-Proof/Init.thy
@@ -2,17 +2,20 @@ theory Init
   imports Host
 begin
 
-definition func_ret_idx :: nat where "func_ret_idx = 11"
-definition func_make_storage_coupon_idx :: nat where "func_make_storage_coupon_idx = 12"
-definition func_make_tree_coupon_idx :: nat where "func_make_tree_coupon_idx = 13"
-definition func_make_thunk_coupon_idx :: nat where "func_make_thunk_coupon_idx = 14"
-definition func_make_thunktree_coupon_idx :: nat where "func_make_thunktree_coupon_idx = 15"
-definition func_make_thunkforce_coupon_idx :: nat where "func_make_thunkforce_coupon_idx = 16"
-definition func_make_encode_coupon_idx :: nat where "func_make_encode_coupon_idx = 17"
-definition func_make_sym_coupon_idx :: nat where "func_make_sym_coupon_idx = 18"
-definition func_make_trans_coupon_idx :: nat where "func_make_trans_coupon_idx = 19"
-definition func_make_self_coupon_idx :: nat where "func_make_self_coupon_idx = 20"
-definition func_make_coupon_idx :: nat where "func_make_coupon_idx = 21"
+definition func_make_eq_tree_coupon_idx :: nat where "func_make_eq_tree_coupon_idx = 21"
+definition func_make_eval_tree_coupon_idx :: nat where "func_make_eval_tree_coupon_idx = 22"
+definition func_make_force_result_eq_coupon_idx :: nat where "func_make_force_result_eq_coupon_idx = 23"
+definition func_make_eval_eq_coupon_idx :: nat where "func_make_eval_eq_coupon_idx = 24"
+definition func_make_think_application_coupon_idx :: nat where "func_make_think_application_coupon_idx = 25"
+definition func_make_think_to_force_coupon_idx :: nat where "func_make_think_to_force_coupon_idx = 26"
+definition func_make_force_to_encode_strict_coupon_idx :: nat where "func_make_force_to_encode_strict_coupon_idx = 27"
+definition func_make_eval_blobobj_coupon_idx :: nat where "func_make_eval_blobobj_coupon_idx = 28"
+definition func_make_eq_application_coupon_idx :: nat where "func_make_eq_application_coupon_idx = 29"
+definition func_make_eq_encode_strict_coupon_idx :: nat where "func_make_eq_encode_strict_coupon_idx = 30"
+definition func_make_sym_coupon_idx :: nat where "func_make_sym_coupon_idx = 31"
+definition func_make_trans_coupon_idx :: nat where "func_make_trans_coupon_idx = 32"
+definition func_make_self_coupon_idx :: nat where "func_make_self_coupon_idx = 33"
+definition func_make_coupon_idx :: nat where "func_make_coupon_idx = 34"
 definition tab_coupons_idx :: nat where "tab_coupons_idx = 0"
 definition init :: "s" where "init = 
 \<lparr> funcs = 
@@ -20,13 +23,23 @@ definition init :: "s" where "init =
 (Func_host ([(T_ref T_ext_ref)] _> [(T_num T_i32)]) (Host_func fixpoint_is_storage_coupon)),
 (Func_host ([(T_ref T_ext_ref)] _> [(T_num T_i32)]) (Host_func fixpoint_is_force_coupon)),
 (Func_host ([(T_ref T_ext_ref)] _> [(T_num T_i32)]) (Host_func fixpoint_is_eq_coupon)),
-(Func_host ([(T_ref T_ext_ref)] _> [(T_ref T_ext_ref)]) (Host_func fixpoint_create_thunk)),
-(Func_host ([(T_ref T_ext_ref)] _> [(T_ref T_ext_ref)]) (Host_func fixpoint_create_encode)),
+(Func_host ([(T_ref T_ext_ref)] _> [(T_num T_i32)]) (Host_func fixpoint_is_eval_coupon)),
+(Func_host ([(T_ref T_ext_ref)] _> [(T_num T_i32)]) (Host_func fixpoint_is_apply_coupon)),
+(Func_host ([(T_ref T_ext_ref)] _> [(T_num T_i32)]) (Host_func fixpoint_is_think_coupon)),
+(Func_host ([(T_ref T_ext_ref)] _> [(T_ref T_ext_ref)]) (Host_func fixpoint_create_application_thunk)),
+(Func_host ([(T_ref T_ext_ref)] _> [(T_ref T_ext_ref)]) (Host_func fixpoint_create_strict_encode)),
+(Func_host ([(T_ref T_ext_ref)] _> [(T_ref T_ext_ref)]) (Host_func fixpoint_create_shallow_encode)),
 (Func_host ([(T_ref T_ext_ref)] _> [(T_ref T_ext_ref)]) (Host_func fixpoint_get_coupon_lhs)),
 (Func_host ([(T_ref T_ext_ref)] _> [(T_ref T_ext_ref)]) (Host_func fixpoint_get_coupon_rhs)),
 (Func_host ([(T_ref T_ext_ref), (T_ref T_ext_ref)] _> [(T_ref T_ext_ref)]) (Host_func fixpoint_create_eq_coupon)),
+(Func_host ([(T_ref T_ext_ref), (T_ref T_ext_ref)] _> [(T_ref T_ext_ref)]) (Host_func fixpoint_create_eval_coupon)),
+(Func_host ([(T_ref T_ext_ref), (T_ref T_ext_ref)] _> [(T_ref T_ext_ref)]) (Host_func fixpoint_create_think_coupon)),
+(Func_host ([(T_ref T_ext_ref), (T_ref T_ext_ref)] _> [(T_ref T_ext_ref)]) (Host_func fixpoint_create_force_coupon)),
 (Func_host ([(T_ref T_ext_ref)] _> [(T_num T_i32)]) (Host_func fixpoint_get_tree_size)),
 (Func_host ([(T_ref T_ext_ref), (T_num T_i32)] _> [(T_ref T_ext_ref)]) (Host_func fixpoint_get_tree_data)),
+(Func_host ([(T_ref T_ext_ref)] _> [(T_num T_i32)]) (Host_func fixpoint_is_blob_obj)),
+(Func_host ([(T_ref T_ext_ref)] _> [(T_num T_i32)]) (Host_func fixpoint_is_data)),
+(Func_host ([(T_ref T_ext_ref)] _> [(T_num T_i32)]) (Host_func fixpoint_is_object)),
 (Func_native 
 \<lparr>types = [([(T_ref T_ext_ref), (T_ref T_ext_ref)] _> [(T_ref T_ext_ref)]),
 ([(T_ref T_ext_ref), (T_ref T_ext_ref)] _> [(T_num T_i32)]),
@@ -34,67 +47,7 @@ definition init :: "s" where "init =
 ([(T_ref T_ext_ref)] _> [(T_ref T_ext_ref)]),
 ([(T_ref T_ext_ref), (T_num T_i32)] _> [(T_ref T_ext_ref)]),
 ([(T_num T_i32), (T_ref T_ext_ref), (T_ref T_ext_ref)] _> [(T_ref T_ext_ref)])],
-funcs = [0, 1, 2, 3, 4, 5, 6, 7, 8, 9, 10, 11, 12, 13, 14, 15, 16, 17, 18, 19, 20, 21],
-tabs = [0, 1],
-mems = [],
-globs = [],
-elems = [0],
-datas = []
-\<rparr>
-([(T_ref T_ext_ref), (T_ref T_ext_ref)] _> [(T_ref T_ext_ref)])
-[]
-[(Local_get 0),
-(Local_get 1),
-(Call 0),
-(If (Tbv (Some (T_ref T_ext_ref)))
-[(Local_get 0)]
-[(Local_get 1)])]),
-(Func_native 
-\<lparr>types = [([(T_ref T_ext_ref), (T_ref T_ext_ref)] _> [(T_ref T_ext_ref)]),
-([(T_ref T_ext_ref), (T_ref T_ext_ref)] _> [(T_num T_i32)]),
-([(T_ref T_ext_ref)] _> [(T_num T_i32)]),
-([(T_ref T_ext_ref)] _> [(T_ref T_ext_ref)]),
-([(T_ref T_ext_ref), (T_num T_i32)] _> [(T_ref T_ext_ref)]),
-([(T_num T_i32), (T_ref T_ext_ref), (T_ref T_ext_ref)] _> [(T_ref T_ext_ref)])],
-funcs = [0, 1, 2, 3, 4, 5, 6, 7, 8, 9, 10, 11, 12, 13, 14, 15, 16, 17, 18, 19, 20, 21],
-tabs = [0, 1],
-mems = [],
-globs = [],
-elems = [0],
-datas = []
-\<rparr>
-([(T_ref T_ext_ref), (T_ref T_ext_ref)] _> [(T_ref T_ext_ref)])
-[(T_ref T_ext_ref)]
-[(EConstNum (ConstInt32 (Abs_i32 0))),
-(Table_get 0),
-(Local_set 2),
-(Local_get 2),
-(Call 1),
-(If (Tbv (Some (T_ref T_ext_ref)))
-[(Local_get 0),
-(Local_get 2),
-(Call 6),
-(Call 0),
-(If (Tbv (Some (T_ref T_ext_ref)))
-[(Local_get 1),
-(Local_get 2),
-(Call 7),
-(Call 0),
-(If (Tbv (Some (T_ref T_ext_ref)))
-[(Local_get 0),
-(Local_get 1),
-(Call 8)]
-[Unreachable])]
-[Unreachable])]
-[Unreachable])]),
-(Func_native 
-\<lparr>types = [([(T_ref T_ext_ref), (T_ref T_ext_ref)] _> [(T_ref T_ext_ref)]),
-([(T_ref T_ext_ref), (T_ref T_ext_ref)] _> [(T_num T_i32)]),
-([(T_ref T_ext_ref)] _> [(T_num T_i32)]),
-([(T_ref T_ext_ref)] _> [(T_ref T_ext_ref)]),
-([(T_ref T_ext_ref), (T_num T_i32)] _> [(T_ref T_ext_ref)]),
-([(T_num T_i32), (T_ref T_ext_ref), (T_ref T_ext_ref)] _> [(T_ref T_ext_ref)])],
-funcs = [0, 1, 2, 3, 4, 5, 6, 7, 8, 9, 10, 11, 12, 13, 14, 15, 16, 17, 18, 19, 20, 21],
+funcs = [0, 1, 2, 3, 4, 5, 6, 7, 8, 9, 10, 11, 12, 13, 14, 15, 16, 17, 18, 19, 20, 21, 22, 23, 24, 25, 26, 27, 28, 29, 30, 31, 32, 33, 34],
 tabs = [0, 1],
 mems = [],
 globs = [],
@@ -125,12 +78,12 @@ datas = []
 (Local_set 4),
 (Br 0)])]),
 (Local_get 0),
-(Call 9),
+(Call 16),
 (Local_get 3),
 (Relop T_i32 (Relop_i relop_i.Eq)),
 (If (Tbv (Some (T_ref T_ext_ref)))
 [(Local_get 1),
-(Call 9),
+(Call 16),
 (Local_get 3),
 (Relop T_i32 (Relop_i relop_i.Eq)),
 (If (Tbv (Some (T_ref T_ext_ref)))
@@ -147,16 +100,16 @@ datas = []
 (Local_set 2),
 (Local_get 0),
 (Local_get 4),
-(Call 10),
+(Call 17),
 (Local_get 2),
-(Call 6),
+(Call 10),
 (Call 0),
 (If (Tbv None)
 [(Local_get 1),
 (Local_get 4),
-(Call 10),
+(Call 17),
 (Local_get 2),
-(Call 7),
+(Call 11),
 (Call 0),
 (If (Tbv None)
 [Nop]
@@ -169,7 +122,7 @@ datas = []
 (Br 0)])]),
 (Local_get 0),
 (Local_get 1),
-(Call 8)]
+(Call 12)]
 [Unreachable])]
 [Unreachable])]),
 (Func_native 
@@ -179,7 +132,92 @@ datas = []
 ([(T_ref T_ext_ref)] _> [(T_ref T_ext_ref)]),
 ([(T_ref T_ext_ref), (T_num T_i32)] _> [(T_ref T_ext_ref)]),
 ([(T_num T_i32), (T_ref T_ext_ref), (T_ref T_ext_ref)] _> [(T_ref T_ext_ref)])],
-funcs = [0, 1, 2, 3, 4, 5, 6, 7, 8, 9, 10, 11, 12, 13, 14, 15, 16, 17, 18, 19, 20, 21],
+funcs = [0, 1, 2, 3, 4, 5, 6, 7, 8, 9, 10, 11, 12, 13, 14, 15, 16, 17, 18, 19, 20, 21, 22, 23, 24, 25, 26, 27, 28, 29, 30, 31, 32, 33, 34],
+tabs = [0, 1],
+mems = [],
+globs = [],
+elems = [0],
+datas = []
+\<rparr>
+([(T_ref T_ext_ref), (T_ref T_ext_ref)] _> [(T_ref T_ext_ref)])
+[(T_ref T_ext_ref), (T_num T_i32), (T_num T_i32)]
+[(Table_size 0),
+(Local_set 3),
+(EConstNum (ConstInt32 (Abs_i32 0))),
+(Local_set 4),
+(Block (Tbv None)
+[(Loop (Tbv None)
+[(Local_get 4),
+(Local_get 3),
+(Relop T_i32 (Relop_i (relop_i.Ge S))),
+(Br_if 1),
+(Local_get 4),
+(Table_get 0),
+(Call 4),
+(If (Tbv None)
+[Nop]
+[Unreachable]),
+(Local_get 4),
+(EConstNum (ConstInt32 (Abs_i32 1))),
+(Binop T_i32 (Binop_i Add)),
+(Local_set 4),
+(Br 0)])]),
+(Local_get 0),
+(Call 16),
+(Local_get 3),
+(Relop T_i32 (Relop_i relop_i.Eq)),
+(If (Tbv (Some (T_ref T_ext_ref)))
+[(Local_get 1),
+(Call 16),
+(Local_get 3),
+(Relop T_i32 (Relop_i relop_i.Eq)),
+(If (Tbv (Some (T_ref T_ext_ref)))
+[(EConstNum (ConstInt32 (Abs_i32 0))),
+(Local_set 4),
+(Block (Tbv None)
+[(Loop (Tbv None)
+[(Local_get 4),
+(Local_get 3),
+(Relop T_i32 (Relop_i (relop_i.Ge S))),
+(Br_if 1),
+(Local_get 4),
+(Table_get 0),
+(Local_set 2),
+(Local_get 0),
+(Local_get 4),
+(Call 17),
+(Local_get 2),
+(Call 10),
+(Call 0),
+(If (Tbv None)
+[(Local_get 1),
+(Local_get 4),
+(Call 17),
+(Local_get 2),
+(Call 11),
+(Call 0),
+(If (Tbv None)
+[Nop]
+[Unreachable])]
+[Unreachable]),
+(Local_get 4),
+(EConstNum (ConstInt32 (Abs_i32 1))),
+(Binop T_i32 (Binop_i Add)),
+(Local_set 4),
+(Br 0)])]),
+(Local_get 0),
+(Local_get 1),
+(Call 13)]
+[Unreachable])]
+[Unreachable])]),
+(Func_native 
+\<lparr>types = [([(T_ref T_ext_ref), (T_ref T_ext_ref)] _> [(T_ref T_ext_ref)]),
+([(T_ref T_ext_ref), (T_ref T_ext_ref)] _> [(T_num T_i32)]),
+([(T_ref T_ext_ref)] _> [(T_num T_i32)]),
+([(T_ref T_ext_ref)] _> [(T_ref T_ext_ref)]),
+([(T_ref T_ext_ref), (T_num T_i32)] _> [(T_ref T_ext_ref)]),
+([(T_num T_i32), (T_ref T_ext_ref), (T_ref T_ext_ref)] _> [(T_ref T_ext_ref)])],
+funcs = [0, 1, 2, 3, 4, 5, 6, 7, 8, 9, 10, 11, 12, 13, 14, 15, 16, 17, 18, 19, 20, 21, 22, 23, 24, 25, 26, 27, 28, 29, 30, 31, 32, 33, 34],
 tabs = [0, 1],
 mems = [],
 globs = [],
@@ -207,30 +245,30 @@ datas = []
 (Call 3),
 (If (Tbv (Some (T_ref T_ext_ref)))
 [(Local_get 2),
-(Call 7),
+(Call 11),
 (Local_get 4),
-(Call 6),
+(Call 10),
 (Call 0),
 (If (Tbv (Some (T_ref T_ext_ref)))
 [(Local_get 3),
-(Call 7),
+(Call 11),
 (Local_get 4),
-(Call 7),
+(Call 11),
 (Call 0),
 (If (Tbv (Some (T_ref T_ext_ref)))
 [(Local_get 2),
-(Call 6),
+(Call 10),
 (Local_get 0),
 (Call 0),
 (If (Tbv (Some (T_ref T_ext_ref)))
 [(Local_get 3),
-(Call 6),
+(Call 10),
 (Local_get 1),
 (Call 0),
 (If (Tbv (Some (T_ref T_ext_ref)))
 [(Local_get 0),
 (Local_get 1),
-(Call 8)]
+(Call 12)]
 [Unreachable])]
 [Unreachable])]
 [Unreachable])]
@@ -245,7 +283,227 @@ datas = []
 ([(T_ref T_ext_ref)] _> [(T_ref T_ext_ref)]),
 ([(T_ref T_ext_ref), (T_num T_i32)] _> [(T_ref T_ext_ref)]),
 ([(T_num T_i32), (T_ref T_ext_ref), (T_ref T_ext_ref)] _> [(T_ref T_ext_ref)])],
-funcs = [0, 1, 2, 3, 4, 5, 6, 7, 8, 9, 10, 11, 12, 13, 14, 15, 16, 17, 18, 19, 20, 21],
+funcs = [0, 1, 2, 3, 4, 5, 6, 7, 8, 9, 10, 11, 12, 13, 14, 15, 16, 17, 18, 19, 20, 21, 22, 23, 24, 25, 26, 27, 28, 29, 30, 31, 32, 33, 34],
+tabs = [0, 1],
+mems = [],
+globs = [],
+elems = [0],
+datas = []
+\<rparr>
+([(T_ref T_ext_ref), (T_ref T_ext_ref)] _> [(T_ref T_ext_ref)])
+[(T_ref T_ext_ref), (T_ref T_ext_ref)]
+[(EConstNum (ConstInt32 (Abs_i32 0))),
+(Table_get 0),
+(Local_set 2),
+(EConstNum (ConstInt32 (Abs_i32 1))),
+(Table_get 0),
+(Local_set 3),
+(Local_get 2),
+(Call 4),
+(If (Tbv (Some (T_ref T_ext_ref)))
+[(Local_get 3),
+(Call 3),
+(If (Tbv (Some (T_ref T_ext_ref)))
+[(Local_get 2),
+(Call 10),
+(Local_get 3),
+(Call 10),
+(Call 0),
+(If (Tbv (Some (T_ref T_ext_ref)))
+[(Local_get 3),
+(Call 11),
+(Local_get 0),
+(Call 0),
+(If (Tbv (Some (T_ref T_ext_ref)))
+[(Local_get 2),
+(Call 11),
+(Local_get 1),
+(Call 0),
+(If (Tbv (Some (T_ref T_ext_ref)))
+[(Local_get 0),
+(Local_get 1),
+(Call 13)]
+[Unreachable])]
+[Unreachable])]
+[Unreachable])]
+[Unreachable])]
+[Unreachable])]),
+(Func_native 
+\<lparr>types = [([(T_ref T_ext_ref), (T_ref T_ext_ref)] _> [(T_ref T_ext_ref)]),
+([(T_ref T_ext_ref), (T_ref T_ext_ref)] _> [(T_num T_i32)]),
+([(T_ref T_ext_ref)] _> [(T_num T_i32)]),
+([(T_ref T_ext_ref)] _> [(T_ref T_ext_ref)]),
+([(T_ref T_ext_ref), (T_num T_i32)] _> [(T_ref T_ext_ref)]),
+([(T_num T_i32), (T_ref T_ext_ref), (T_ref T_ext_ref)] _> [(T_ref T_ext_ref)])],
+funcs = [0, 1, 2, 3, 4, 5, 6, 7, 8, 9, 10, 11, 12, 13, 14, 15, 16, 17, 18, 19, 20, 21, 22, 23, 24, 25, 26, 27, 28, 29, 30, 31, 32, 33, 34],
+tabs = [0, 1],
+mems = [],
+globs = [],
+elems = [0],
+datas = []
+\<rparr>
+([(T_ref T_ext_ref), (T_ref T_ext_ref)] _> [(T_ref T_ext_ref)])
+[(T_ref T_ext_ref), (T_ref T_ext_ref)]
+[(EConstNum (ConstInt32 (Abs_i32 0))),
+(Table_get 0),
+(Local_set 2),
+(EConstNum (ConstInt32 (Abs_i32 1))),
+(Table_get 0),
+(Local_set 3),
+(Local_get 2),
+(Call 4),
+(If (Tbv (Some (T_ref T_ext_ref)))
+[(Local_get 3),
+(Call 5),
+(If (Tbv (Some (T_ref T_ext_ref)))
+[(Local_get 2),
+(Call 11),
+(Local_get 3),
+(Call 10),
+(Call 0),
+(If (Tbv (Some (T_ref T_ext_ref)))
+[(Local_get 2),
+(Call 10),
+(Call 7),
+(Local_get 0),
+(Call 0),
+(If (Tbv (Some (T_ref T_ext_ref)))
+[(Local_get 3),
+(Call 11),
+(Local_get 1),
+(Call 0),
+(If (Tbv (Some (T_ref T_ext_ref)))
+[(Local_get 0),
+(Local_get 1),
+(Call 14)]
+[Unreachable])]
+[Unreachable])]
+[Unreachable])]
+[Unreachable])]
+[Unreachable])]),
+(Func_native 
+\<lparr>types = [([(T_ref T_ext_ref), (T_ref T_ext_ref)] _> [(T_ref T_ext_ref)]),
+([(T_ref T_ext_ref), (T_ref T_ext_ref)] _> [(T_num T_i32)]),
+([(T_ref T_ext_ref)] _> [(T_num T_i32)]),
+([(T_ref T_ext_ref)] _> [(T_ref T_ext_ref)]),
+([(T_ref T_ext_ref), (T_num T_i32)] _> [(T_ref T_ext_ref)]),
+([(T_num T_i32), (T_ref T_ext_ref), (T_ref T_ext_ref)] _> [(T_ref T_ext_ref)])],
+funcs = [0, 1, 2, 3, 4, 5, 6, 7, 8, 9, 10, 11, 12, 13, 14, 15, 16, 17, 18, 19, 20, 21, 22, 23, 24, 25, 26, 27, 28, 29, 30, 31, 32, 33, 34],
+tabs = [0, 1],
+mems = [],
+globs = [],
+elems = [0],
+datas = []
+\<rparr>
+([(T_ref T_ext_ref), (T_ref T_ext_ref)] _> [(T_ref T_ext_ref)])
+[(T_ref T_ext_ref)]
+[(EConstNum (ConstInt32 (Abs_i32 0))),
+(Table_get 0),
+(Local_set 2),
+(Local_get 2),
+(Call 6),
+(If (Tbv (Some (T_ref T_ext_ref)))
+[(Local_get 2),
+(Call 11),
+(Call 19),
+(If (Tbv (Some (T_ref T_ext_ref)))
+[(Local_get 2),
+(Call 10),
+(Local_get 0),
+(Call 0),
+(If (Tbv (Some (T_ref T_ext_ref)))
+[(Local_get 2),
+(Call 11),
+(Local_get 1),
+(Call 0),
+(If (Tbv (Some (T_ref T_ext_ref)))
+[(Local_get 0),
+(Local_get 1),
+(Call 15)]
+[Unreachable])]
+[Unreachable])]
+[Unreachable])]
+[Unreachable])]),
+(Func_native 
+\<lparr>types = [([(T_ref T_ext_ref), (T_ref T_ext_ref)] _> [(T_ref T_ext_ref)]),
+([(T_ref T_ext_ref), (T_ref T_ext_ref)] _> [(T_num T_i32)]),
+([(T_ref T_ext_ref)] _> [(T_num T_i32)]),
+([(T_ref T_ext_ref)] _> [(T_ref T_ext_ref)]),
+([(T_ref T_ext_ref), (T_num T_i32)] _> [(T_ref T_ext_ref)]),
+([(T_num T_i32), (T_ref T_ext_ref), (T_ref T_ext_ref)] _> [(T_ref T_ext_ref)])],
+funcs = [0, 1, 2, 3, 4, 5, 6, 7, 8, 9, 10, 11, 12, 13, 14, 15, 16, 17, 18, 19, 20, 21, 22, 23, 24, 25, 26, 27, 28, 29, 30, 31, 32, 33, 34],
+tabs = [0, 1],
+mems = [],
+globs = [],
+elems = [0],
+datas = []
+\<rparr>
+([(T_ref T_ext_ref), (T_ref T_ext_ref)] _> [(T_ref T_ext_ref)])
+[(T_ref T_ext_ref)]
+[(EConstNum (ConstInt32 (Abs_i32 0))),
+(Table_get 0),
+(Local_set 2),
+(Local_get 2),
+(Call 2),
+(If (Tbv (Some (T_ref T_ext_ref)))
+[(Local_get 2),
+(Call 11),
+(Call 20),
+(If (Tbv (Some (T_ref T_ext_ref)))
+[(Local_get 2),
+(Call 11),
+(Local_get 1),
+(Call 0),
+(If (Tbv (Some (T_ref T_ext_ref)))
+[(Local_get 2),
+(Call 10),
+(Call 8),
+(Local_get 0),
+(Call 0),
+(If (Tbv (Some (T_ref T_ext_ref)))
+[(Local_get 0),
+(Local_get 1),
+(Call 12)]
+[Unreachable])]
+[Unreachable])]
+[Unreachable])]
+[Unreachable])]),
+(Func_native 
+\<lparr>types = [([(T_ref T_ext_ref), (T_ref T_ext_ref)] _> [(T_ref T_ext_ref)]),
+([(T_ref T_ext_ref), (T_ref T_ext_ref)] _> [(T_num T_i32)]),
+([(T_ref T_ext_ref)] _> [(T_num T_i32)]),
+([(T_ref T_ext_ref)] _> [(T_ref T_ext_ref)]),
+([(T_ref T_ext_ref), (T_num T_i32)] _> [(T_ref T_ext_ref)]),
+([(T_num T_i32), (T_ref T_ext_ref), (T_ref T_ext_ref)] _> [(T_ref T_ext_ref)])],
+funcs = [0, 1, 2, 3, 4, 5, 6, 7, 8, 9, 10, 11, 12, 13, 14, 15, 16, 17, 18, 19, 20, 21, 22, 23, 24, 25, 26, 27, 28, 29, 30, 31, 32, 33, 34],
+tabs = [0, 1],
+mems = [],
+globs = [],
+elems = [0],
+datas = []
+\<rparr>
+([(T_ref T_ext_ref), (T_ref T_ext_ref)] _> [(T_ref T_ext_ref)])
+[]
+[(Local_get 0),
+(Call 18),
+(If (Tbv (Some (T_ref T_ext_ref)))
+[(Local_get 0),
+(Local_get 1),
+(Call 0),
+(If (Tbv (Some (T_ref T_ext_ref)))
+[(Local_get 0),
+(Local_get 1),
+(Call 13)]
+[Unreachable])]
+[Unreachable])]),
+(Func_native 
+\<lparr>types = [([(T_ref T_ext_ref), (T_ref T_ext_ref)] _> [(T_ref T_ext_ref)]),
+([(T_ref T_ext_ref), (T_ref T_ext_ref)] _> [(T_num T_i32)]),
+([(T_ref T_ext_ref)] _> [(T_num T_i32)]),
+([(T_ref T_ext_ref)] _> [(T_ref T_ext_ref)]),
+([(T_ref T_ext_ref), (T_num T_i32)] _> [(T_ref T_ext_ref)]),
+([(T_num T_i32), (T_ref T_ext_ref), (T_ref T_ext_ref)] _> [(T_ref T_ext_ref)])],
+funcs = [0, 1, 2, 3, 4, 5, 6, 7, 8, 9, 10, 11, 12, 13, 14, 15, 16, 17, 18, 19, 20, 21, 22, 23, 24, 25, 26, 27, 28, 29, 30, 31, 32, 33, 34],
 tabs = [0, 1],
 mems = [],
 globs = [],
@@ -262,19 +520,19 @@ datas = []
 (If (Tbv (Some (T_ref T_ext_ref)))
 [(Local_get 0),
 (Local_get 2),
-(Call 6),
-(Call 4),
+(Call 10),
+(Call 7),
 (Call 0),
 (If (Tbv (Some (T_ref T_ext_ref)))
 [(Local_get 1),
 (Local_get 2),
+(Call 11),
 (Call 7),
-(Call 4),
 (Call 0),
 (If (Tbv (Some (T_ref T_ext_ref)))
 [(Local_get 0),
 (Local_get 1),
-(Call 8)]
+(Call 12)]
 [Unreachable])]
 [Unreachable])]
 [Unreachable])]),
@@ -285,73 +543,7 @@ datas = []
 ([(T_ref T_ext_ref)] _> [(T_ref T_ext_ref)]),
 ([(T_ref T_ext_ref), (T_num T_i32)] _> [(T_ref T_ext_ref)]),
 ([(T_num T_i32), (T_ref T_ext_ref), (T_ref T_ext_ref)] _> [(T_ref T_ext_ref)])],
-funcs = [0, 1, 2, 3, 4, 5, 6, 7, 8, 9, 10, 11, 12, 13, 14, 15, 16, 17, 18, 19, 20, 21],
-tabs = [0, 1],
-mems = [],
-globs = [],
-elems = [0],
-datas = []
-\<rparr>
-([(T_ref T_ext_ref), (T_ref T_ext_ref)] _> [(T_ref T_ext_ref)])
-[(T_ref T_ext_ref), (T_ref T_ext_ref), (T_ref T_ext_ref)]
-[(EConstNum (ConstInt32 (Abs_i32 0))),
-(Table_get 0),
-(Local_set 4),
-(EConstNum (ConstInt32 (Abs_i32 1))),
-(Table_get 0),
-(Local_set 2),
-(EConstNum (ConstInt32 (Abs_i32 2))),
-(Table_get 0),
-(Local_set 3),
-(Local_get 4),
-(Call 3),
-(If (Tbv (Some (T_ref T_ext_ref)))
-[(Local_get 2),
-(Call 2),
-(If (Tbv (Some (T_ref T_ext_ref)))
-[(Local_get 3),
-(Call 2),
-(If (Tbv (Some (T_ref T_ext_ref)))
-[(Local_get 2),
-(Call 6),
-(Local_get 4),
-(Call 6),
-(Call 0),
-(If (Tbv (Some (T_ref T_ext_ref)))
-[(Local_get 3),
-(Call 6),
-(Local_get 4),
-(Call 7),
-(Call 0),
-(If (Tbv (Some (T_ref T_ext_ref)))
-[(Local_get 2),
-(Call 7),
-(Local_get 0),
-(Call 0),
-(If (Tbv (Some (T_ref T_ext_ref)))
-[(Local_get 3),
-(Call 7),
-(Local_get 1),
-(Call 0),
-(If (Tbv (Some (T_ref T_ext_ref)))
-[(Local_get 0),
-(Local_get 1),
-(Call 8)]
-[Unreachable])]
-[Unreachable])]
-[Unreachable])]
-[Unreachable])]
-[Unreachable])]
-[Unreachable])]
-[Unreachable])]),
-(Func_native 
-\<lparr>types = [([(T_ref T_ext_ref), (T_ref T_ext_ref)] _> [(T_ref T_ext_ref)]),
-([(T_ref T_ext_ref), (T_ref T_ext_ref)] _> [(T_num T_i32)]),
-([(T_ref T_ext_ref)] _> [(T_num T_i32)]),
-([(T_ref T_ext_ref)] _> [(T_ref T_ext_ref)]),
-([(T_ref T_ext_ref), (T_num T_i32)] _> [(T_ref T_ext_ref)]),
-([(T_num T_i32), (T_ref T_ext_ref), (T_ref T_ext_ref)] _> [(T_ref T_ext_ref)])],
-funcs = [0, 1, 2, 3, 4, 5, 6, 7, 8, 9, 10, 11, 12, 13, 14, 15, 16, 17, 18, 19, 20, 21],
+funcs = [0, 1, 2, 3, 4, 5, 6, 7, 8, 9, 10, 11, 12, 13, 14, 15, 16, 17, 18, 19, 20, 21, 22, 23, 24, 25, 26, 27, 28, 29, 30, 31, 32, 33, 34],
 tabs = [0, 1],
 mems = [],
 globs = [],
@@ -367,20 +559,20 @@ datas = []
 (Call 3),
 (If (Tbv (Some (T_ref T_ext_ref)))
 [(Local_get 2),
-(Call 6),
-(Call 5),
+(Call 10),
+(Call 8),
 (Local_get 0),
 (Call 0),
 (If (Tbv (Some (T_ref T_ext_ref)))
 [(Local_get 2),
-(Call 7),
-(Call 5),
+(Call 11),
+(Call 8),
 (Local_get 1),
 (Call 0),
 (If (Tbv (Some (T_ref T_ext_ref)))
 [(Local_get 0),
 (Local_get 1),
-(Call 8)]
+(Call 12)]
 [Unreachable])]
 [Unreachable])]
 [Unreachable])]),
@@ -391,7 +583,7 @@ datas = []
 ([(T_ref T_ext_ref)] _> [(T_ref T_ext_ref)]),
 ([(T_ref T_ext_ref), (T_num T_i32)] _> [(T_ref T_ext_ref)]),
 ([(T_num T_i32), (T_ref T_ext_ref), (T_ref T_ext_ref)] _> [(T_ref T_ext_ref)])],
-funcs = [0, 1, 2, 3, 4, 5, 6, 7, 8, 9, 10, 11, 12, 13, 14, 15, 16, 17, 18, 19, 20, 21],
+funcs = [0, 1, 2, 3, 4, 5, 6, 7, 8, 9, 10, 11, 12, 13, 14, 15, 16, 17, 18, 19, 20, 21, 22, 23, 24, 25, 26, 27, 28, 29, 30, 31, 32, 33, 34],
 tabs = [0, 1],
 mems = [],
 globs = [],
@@ -407,18 +599,18 @@ datas = []
 (Call 3),
 (If (Tbv (Some (T_ref T_ext_ref)))
 [(Local_get 2),
-(Call 7),
+(Call 11),
 (Local_get 0),
 (Call 0),
 (If (Tbv (Some (T_ref T_ext_ref)))
 [(Local_get 2),
-(Call 6),
+(Call 10),
 (Local_get 1),
 (Call 0),
 (If (Tbv (Some (T_ref T_ext_ref)))
 [(Local_get 0),
 (Local_get 1),
-(Call 8)]
+(Call 12)]
 [Unreachable])]
 [Unreachable])]
 [Unreachable])]),
@@ -429,7 +621,7 @@ datas = []
 ([(T_ref T_ext_ref)] _> [(T_ref T_ext_ref)]),
 ([(T_ref T_ext_ref), (T_num T_i32)] _> [(T_ref T_ext_ref)]),
 ([(T_num T_i32), (T_ref T_ext_ref), (T_ref T_ext_ref)] _> [(T_ref T_ext_ref)])],
-funcs = [0, 1, 2, 3, 4, 5, 6, 7, 8, 9, 10, 11, 12, 13, 14, 15, 16, 17, 18, 19, 20, 21],
+funcs = [0, 1, 2, 3, 4, 5, 6, 7, 8, 9, 10, 11, 12, 13, 14, 15, 16, 17, 18, 19, 20, 21, 22, 23, 24, 25, 26, 27, 28, 29, 30, 31, 32, 33, 34],
 tabs = [0, 1],
 mems = [],
 globs = [],
@@ -451,24 +643,24 @@ datas = []
 (Call 3),
 (If (Tbv (Some (T_ref T_ext_ref)))
 [(Local_get 2),
-(Call 7),
+(Call 11),
 (Local_get 3),
-(Call 6),
+(Call 10),
 (Call 0),
 (If (Tbv (Some (T_ref T_ext_ref)))
 [(Local_get 0),
 (Local_get 2),
-(Call 6),
+(Call 10),
 (Call 0),
 (If (Tbv (Some (T_ref T_ext_ref)))
 [(Local_get 1),
 (Local_get 3),
-(Call 7),
+(Call 11),
 (Call 0),
 (If (Tbv (Some (T_ref T_ext_ref)))
 [(Local_get 0),
 (Local_get 1),
-(Call 8)]
+(Call 12)]
 [Unreachable])]
 [Unreachable])]
 [Unreachable])]
@@ -481,7 +673,7 @@ datas = []
 ([(T_ref T_ext_ref)] _> [(T_ref T_ext_ref)]),
 ([(T_ref T_ext_ref), (T_num T_i32)] _> [(T_ref T_ext_ref)]),
 ([(T_num T_i32), (T_ref T_ext_ref), (T_ref T_ext_ref)] _> [(T_ref T_ext_ref)])],
-funcs = [0, 1, 2, 3, 4, 5, 6, 7, 8, 9, 10, 11, 12, 13, 14, 15, 16, 17, 18, 19, 20, 21],
+funcs = [0, 1, 2, 3, 4, 5, 6, 7, 8, 9, 10, 11, 12, 13, 14, 15, 16, 17, 18, 19, 20, 21, 22, 23, 24, 25, 26, 27, 28, 29, 30, 31, 32, 33, 34],
 tabs = [0, 1],
 mems = [],
 globs = [],
@@ -496,7 +688,7 @@ datas = []
 (If (Tbv (Some (T_ref T_ext_ref)))
 [(Local_get 0),
 (Local_get 1),
-(Call 8)]
+(Call 12)]
 [Unreachable])]),
 (Func_native 
 \<lparr>types = [([(T_ref T_ext_ref), (T_ref T_ext_ref)] _> [(T_ref T_ext_ref)]),
@@ -505,7 +697,7 @@ datas = []
 ([(T_ref T_ext_ref)] _> [(T_ref T_ext_ref)]),
 ([(T_ref T_ext_ref), (T_num T_i32)] _> [(T_ref T_ext_ref)]),
 ([(T_num T_i32), (T_ref T_ext_ref), (T_ref T_ext_ref)] _> [(T_ref T_ext_ref)])],
-funcs = [0, 1, 2, 3, 4, 5, 6, 7, 8, 9, 10, 11, 12, 13, 14, 15, 16, 17, 18, 19, 20, 21],
+funcs = [0, 1, 2, 3, 4, 5, 6, 7, 8, 9, 10, 11, 12, 13, 14, 15, 16, 17, 18, 19, 20, 21, 22, 23, 24, 25, 26, 27, 28, 29, 30, 31, 32, 33, 34],
 tabs = [0, 1],
 mems = [],
 globs = [],
@@ -524,15 +716,19 @@ datas = []
 (Call_indirect 1 0)]
 [Unreachable])])],
 tabs = [((T_tab \<lparr> l_min = 0, l_max = None\<rparr> T_ext_ref), []),
-((T_tab \<lparr> l_min = 9, l_max = (Some 9)\<rparr> T_func_ref), [(ConstRefFunc 12),
-(ConstRefFunc 13),
-(ConstRefFunc 14),
-(ConstRefFunc 15),
-(ConstRefFunc 16),
-(ConstRefFunc 17),
-(ConstRefFunc 18),
-(ConstRefFunc 19),
-(ConstRefFunc 20)])],
+((T_tab \<lparr> l_min = 13, l_max = (Some 13)\<rparr> T_func_ref), [(ConstRefFunc 21),
+(ConstRefFunc 29),
+(ConstRefFunc 23),
+(ConstRefFunc 30),
+(ConstRefFunc 25),
+(ConstRefFunc 26),
+(ConstRefFunc 27),
+(ConstRefFunc 24),
+(ConstRefFunc 28),
+(ConstRefFunc 22),
+(ConstRefFunc 31),
+(ConstRefFunc 32),
+(ConstRefFunc 33)])],
 mems = [],
 globs = [],
 elems = [],
