wasm-proofs/Wasm-Proof/eval_blobobj_coupon.thy
@@ -1,0 +1,110 @@
+theory eval_blobobj_coupon
+  imports custom_method isabelle_coupon
+begin
+
+lemma make_some:
+  assumes "make_eval_blob_coupon coupons l r = Some res"
+  shows "get_type l = 0 \<and> is_equal l r \<and> res = create_coupon Eval l r"
+  by (metis assms if_Some_None_eq_None make_eval_blob_coupon.simps
+      option.inject)
+
+lemma make_none:
+  assumes "make_eval_blob_coupon coupons l r = None" 
+  shows "\<not> get_type l = 0 \<or> \<not>is_equal l r "
+  using assms by force
+
+lemma plus_20:
+"n + 20 = (Suc (Suc (Suc (Suc (Suc (Suc (Suc (Suc (Suc (Suc (Suc (Suc (Suc (Suc (Suc (Suc (Suc (Suc (Suc (Suc n))))))))))))))))))))"
+  by auto
+
+lemma make_eval_blob_coupon_run_iter:
+  assumes "make_eval_blob_coupon coupons l r = Some res"
+  shows  "run_iter (n + 20)
+          (Config 
+           (Suc n')
+           (init\<lparr> tabs := (tabs init)[tab_coupons_idx := ((T_tab \<lparr> l_min = 0, l_max = None\<rparr> T_ext_ref), (map (\<lambda>c. (ConstRefExtern (to_externref c))) coupons))] \<rparr>)
+           (Frame_context 
+              (Redex ((V_ref (ConstRefExtern (to_externref r))) #
+                      (V_ref (ConstRefExtern (to_externref l))) #
+                      rest_vs)
+                     [Invoke func_make_eval_blobobj_coupon_idx]
+                     b_es)
+            lc f \<lparr>f_locs = locs, f_inst = exp_inst\<rparr>) fcs)
+ =
+          run_iter n
+          (Config 
+           (Suc n')
+           (init\<lparr> tabs := (tabs init)[tab_coupons_idx := ((T_tab \<lparr> l_min = 0, l_max = None\<rparr> T_ext_ref), (map (\<lambda>c. (ConstRefExtern (to_externref c))) coupons))] \<rparr>)
+            (Frame_context (Redex (V_ref (ConstRefExtern (to_externref res)) # rest_vs) [] b_es) lc f  \<lparr>f_locs = locs, f_inst = exp_inst\<rparr>) fcs)"
+proof -
+  let ?state = " (init\<lparr> tabs := (tabs init)[tab_coupons_idx := ((T_tab \<lparr> l_min = 0, l_max = None\<rparr> T_ext_ref), (map (\<lambda>c. (ConstRefExtern (to_externref c))) coupons))] \<rparr> )"
+
+  have "get_type r = 0"
+    using make_some[OF assms]
+    by auto
+
+  then show ?thesis
+    using make_some[OF assms]
+          fixpoint_is_equal_impl[of ?state]
+          fixpoint_create_eval_coupon_impl[of ?state]
+          fixpoint_is_blob_obj_impl[of ?state]
+    apply (invoke_coupon_func fuel_idx_def: plus_20 func_make_eval_blobobj_coupon_idx_def)
+    apply (call_api_func)
+    apply (if_block)
+    apply (call_api_func)
+    apply (if_block)
+    apply (call_api_func)
+    done
+qed
+
+lemma make_eval_blobobj_coupon_run_invoke_none:
+  assumes "make_eval_blob_coupon coupons l r = None"
+  shows "\<exists>msg cfg.
+         run_iter (n + 20)
+          (Config 
+           (Suc n')
+           (init\<lparr> tabs := (tabs init)[tab_coupons_idx := ((T_tab \<lparr> l_min = 0, l_max = None\<rparr> T_ext_ref), (map (\<lambda>c. (ConstRefExtern (to_externref c))) coupons))] \<rparr>)
+           (Frame_context 
+              (Redex ((V_ref (ConstRefExtern (to_externref r))) #
+                      (V_ref (ConstRefExtern (to_externref l))) #
+                      rest_vs)
+                     [Invoke func_make_eval_blobobj_coupon_idx]
+                     b_es)
+            lc f \<lparr>f_locs = locs, f_inst = exp_inst\<rparr>) fcs)
+ = (cfg, RTrap msg)"
+proof -
+  let ?A = "\<not>get_type l = 0"
+  let ?B = "get_type l = 0 \<and> \<not>is_equal l r"
+
+  let ?state = "(init\<lparr> tabs := (tabs init)[tab_coupons_idx := ((T_tab \<lparr> l_min = 0, l_max = None\<rparr> T_ext_ref), (map (\<lambda>c. (ConstRefExtern (to_externref c))) coupons))] \<rparr>)"
+
+  have assms: "?A \<or> ?B" 
+    using make_none[OF assms] 
+    by meson
+
+  show ?thesis
+    using assms
+  proof
+    assume ?A
+    then show ?thesis
+      using fixpoint_is_blob_obj_impl[of ?state]
+      apply (invoke_coupon_func fuel_idx_def: plus_20 func_make_eval_blobobj_coupon_idx_def)
+      apply (call_api_func)
+      apply (if_block)
+      done
+  next
+    assume ?B
+    then show ?thesis
+      using fixpoint_is_equal_impl[of ?state]
+            fixpoint_create_eval_coupon_impl[of ?state]
+            fixpoint_is_blob_obj_impl[of ?state]
+      apply (invoke_coupon_func fuel_idx_def: plus_20 func_make_eval_blobobj_coupon_idx_def)
+      apply (call_api_func)
+      apply (if_block)
+      apply (call_api_func)
+      apply (if_block)
+      done
+  qed
+qed
+
+end
