wasm-proofs/Wasm-Proof/force_to_encode_strict_coupon.thy
@@ -1,0 +1,300 @@
+theory force_to_encode_strict_coupon
+  imports custom_method isabelle_coupon
+begin
+
+lemma make_some:
+  assumes "make_force_to_encode_strict_coupon coupons l r = Some res"
+  shows "\<exists>t xs tl.
+         coupons = t # xs
+       \<and> is_force_coupon t
+       \<and> get_coupon_lhs t = Some tl
+       \<and> get_coupon_rhs t = Some r
+       \<and> create_strict_encode_api tl = Some l
+       \<and> (get_type r = 0 \<or> get_type r = 1)
+       \<and> res = create_coupon Eq l r"
+proof -
+  obtain t xs where 1: "coupons = t # xs \<and> is_force_coupon t"
+    using assms
+    apply (cases coupons; simp_all)
+    by fastforce
+
+  then obtain tl tr where 2: "get_coupon_lhs t = Some tl \<and> get_coupon_rhs t = Some tr"
+    using force_lhs_exist force_rhs_exist
+    by presburger
+
+  show ?thesis
+    using 1 2 assms
+    apply simp
+    apply (cases "create_strict_encode_api tl"; simp_all)
+    by (metis option.distinct(1) option.sel)
+qed
+
+lemma make_none:
+  assumes "make_force_to_encode_strict_coupon coupons l r = None" 
+  shows "(length coupons = 0) \<or>
+         (\<exists>t xs. coupons = t # xs \<and> \<not> is_force_coupon t) \<or>
+         (\<exists>t xs tl tr. 
+           coupons = t # xs 
+         \<and> is_force_coupon t
+         \<and> get_coupon_lhs t = Some tl
+         \<and> get_coupon_rhs t = Some tr
+         \<and> create_strict_encode_api tl = None) \<or>
+         (\<exists>t xs tl tr encode. 
+           coupons = t # xs 
+         \<and> is_force_coupon t
+         \<and> get_coupon_lhs t = Some tl
+         \<and> get_coupon_rhs t = Some tr
+         \<and> create_strict_encode_api tl = Some encode
+         \<and> ((get_type tr = 0 \<or> get_type tr = 1) \<longrightarrow> (\<not> is_equal encode l \<or> \<not> is_equal tr r)))"
+proof (cases "length coupons = 0")
+  case True then show ?thesis by auto
+next
+  case False
+  then obtain t xs where 1: "coupons = t # xs"
+    by (metis list.exhaust list.size(3))
+  then show ?thesis
+  proof (cases "is_force_coupon t")
+    case False then show ?thesis
+      using 1 by blast
+  next
+    case True
+    then obtain tl tr where
+         "get_coupon_lhs t = Some tl
+        \<and> get_coupon_rhs t = Some tr"
+      using force_lhs_exist force_rhs_exist
+      by presburger
+
+    then show ?thesis
+      using 1 assms
+      by fastforce
+  qed
+qed
+
+lemma plus_43:
+"n + 43 = (Suc (Suc (Suc (Suc (Suc (Suc (Suc (Suc (Suc (Suc (Suc (Suc (Suc 
+(Suc (Suc (Suc (Suc (Suc (Suc (Suc(Suc (Suc (Suc (Suc (Suc (Suc (Suc (Suc (Suc (Suc (Suc (Suc (Suc (Suc (Suc (Suc (Suc (Suc (Suc (Suc (Suc (Suc (Suc n)))))))))))))))))))))))))))))))))))))))))))"
+  by auto
+
+lemma make_force_to_encode_strict_coupon_run_iter:
+  assumes "make_force_to_encode_strict_coupon coupons l r = Some res"
+  shows  "run_iter (n + 43)
+          (Config 
+           (Suc n')
+           (init\<lparr> tabs := (tabs init)[tab_coupons_idx := ((T_tab \<lparr> l_min = 0, l_max = None\<rparr> T_ext_ref), (map (\<lambda>c. (ConstRefExtern (to_externref c))) coupons))] \<rparr>)
+           (Frame_context 
+              (Redex ((V_ref (ConstRefExtern (to_externref r))) #
+                      (V_ref (ConstRefExtern (to_externref l))) #
+                      rest_vs)
+                     [Invoke func_make_force_to_encode_strict_coupon_idx]
+                     b_es)
+            lc f \<lparr>f_locs = locs, f_inst = exp_inst\<rparr>) fcs)
+ =
+          run_iter n
+          (Config 
+           (Suc n')
+           (init\<lparr> tabs := (tabs init)[tab_coupons_idx := ((T_tab \<lparr> l_min = 0, l_max = None\<rparr> T_ext_ref), (map (\<lambda>c. (ConstRefExtern (to_externref c))) coupons))] \<rparr>)
+            (Frame_context (Redex (V_ref (ConstRefExtern (to_externref res)) # rest_vs) [] b_es) lc f  \<lparr>f_locs = locs, f_inst = exp_inst\<rparr>) fcs)"
+proof -
+  obtain t xs tl where
+         1: "coupons = t # xs
+       \<and> is_force_coupon t
+       \<and> get_coupon_lhs t = Some tl
+       \<and> get_coupon_rhs t = Some r
+       \<and> create_strict_encode_api tl = Some l
+       \<and> (get_type r = 0 \<or> get_type r = 1)
+       \<and> res = create_coupon Eq l r"
+    using make_some[OF assms] by auto
+
+  let ?state = " (init\<lparr> tabs := (tabs init)[tab_coupons_idx := ((T_tab \<lparr> l_min = 0, l_max = None\<rparr> T_ext_ref), (map (\<lambda>c. (ConstRefExtern (to_externref c))) coupons))] \<rparr> )"
+
+  show ?thesis
+    using 1 
+          fixpoint_is_force_coupon_impl[of ?state]
+          fixpoint_get_coupon_lhs_impl[of ?state]
+          fixpoint_get_coupon_rhs_impl[of ?state]
+          fixpoint_is_equal_impl[of ?state]
+          fixpoint_is_object_impl[of ?state]
+          fixpoint_create_eq_coupon_impl[of ?state]
+          fixpoint_create_strict_encode_impl[of ?state]
+    apply (invoke_coupon_func fuel_idx_def: plus_43 func_make_force_to_encode_strict_coupon_idx_def)
+    apply (table_get_local_set)
+    apply (call_api_func)
+    apply (if_block)
+    apply (call_api_func)
+    apply (if_block)
+    apply (call_api_func)
+    apply (if_block)
+    apply (call_api_func)
+    apply (if_block)
+    apply (call_api_func)
+    done
+qed
+
+lemma make_force_to_encode_strict_coupon_run_invoke_none:
+  assumes "make_force_to_encode_strict_coupon coupons l r = None"
+  shows "\<exists>msg cfg.
+         run_iter (n + 43)
+          (Config 
+           (Suc n')
+           (init\<lparr> tabs := (tabs init)[tab_coupons_idx := ((T_tab \<lparr> l_min = 0, l_max = None\<rparr> T_ext_ref), (map (\<lambda>c. (ConstRefExtern (to_externref c))) coupons))] \<rparr>)
+           (Frame_context 
+              (Redex ((V_ref (ConstRefExtern (to_externref r))) #
+                      (V_ref (ConstRefExtern (to_externref l))) #
+                      rest_vs)
+                     [Invoke func_make_force_to_encode_strict_coupon_idx]
+                     b_es)
+            lc f \<lparr>f_locs = locs, f_inst = exp_inst\<rparr>) fcs)
+ = (cfg, RTrap msg)"
+proof -
+  let ?A = "(length coupons = 0)"
+  let ?B = "(\<exists>t xs. coupons = t # xs \<and> \<not> is_force_coupon t)"
+  let ?C = "(\<exists>t xs tl tr. 
+           coupons = t # xs 
+         \<and> is_force_coupon t
+         \<and> get_coupon_lhs t = Some tl
+         \<and> get_coupon_rhs t = Some tr
+         \<and> create_strict_encode_api tl = None)"
+  let ?D = "(\<exists>t xs tl tr encode. 
+           coupons = t # xs 
+         \<and> is_force_coupon t
+         \<and> get_coupon_lhs t = Some tl
+         \<and> get_coupon_rhs t = Some tr
+         \<and> create_strict_encode_api tl = Some encode
+         \<and> ((get_type tr = 0 \<or> get_type tr = 1) \<longrightarrow> (\<not> is_equal encode l \<or> \<not> is_equal tr r)))"
+
+  let ?state = "(init\<lparr> tabs := (tabs init)[tab_coupons_idx := ((T_tab \<lparr> l_min = 0, l_max = None\<rparr> T_ext_ref), (map (\<lambda>c. (ConstRefExtern (to_externref c))) coupons))] \<rparr>)"
+
+  have assms: "?A \<or> ?B \<or> ?C \<or> ?D" 
+    using make_none[OF assms] by blast
+
+  show ?thesis
+    using assms
+  proof
+    assume ?A
+    then have "\<not> nat_of_int (I32.lift0 0) < length coupons"
+      by (simp add: nat_of_int_i32.abs_eq)
+    then show ?thesis
+      apply (invoke_coupon_func fuel_idx_def: plus_43 func_make_force_to_encode_strict_coupon_idx_def)
+      apply (table_get_local_set)
+      done
+  next
+    assume "?B \<or> ?C \<or> ?D"
+    then show ?thesis
+    proof
+      assume ?B
+      then obtain t xs where
+        "coupons = t # xs"
+     and "\<not>is_force_coupon t" by blast
+
+      then show ?thesis
+        using fixpoint_is_force_coupon_impl[of ?state]
+        apply (invoke_coupon_func fuel_idx_def: plus_43 func_make_force_to_encode_strict_coupon_idx_def)
+        apply (table_get_local_set)
+        apply (call_api_func)
+        apply (if_block)
+        done
+    next
+      assume "?C \<or> ?D"
+      then show ?thesis
+      proof
+        assume ?C
+        then obtain t xs tl tr where
+           "coupons = t # xs 
+         \<and> is_force_coupon t
+         \<and> get_coupon_lhs t = Some tl
+         \<and> get_coupon_rhs t = Some tr
+         \<and> create_strict_encode_api tl = None"
+          by blast
+        
+        then show ?thesis
+          using fixpoint_is_force_coupon_impl[of ?state]
+            fixpoint_get_coupon_lhs_impl[of ?state]
+            fixpoint_get_coupon_rhs_impl[of ?state]
+            fixpoint_is_equal_impl[of ?state]
+            fixpoint_is_object_impl[of ?state]
+            fixpoint_create_eq_coupon_impl[of ?state]
+            fixpoint_create_strict_encode_impl[of ?state]
+          apply (invoke_coupon_func fuel_idx_def: plus_43 func_make_force_to_encode_strict_coupon_idx_def)
+          apply (table_get_local_set)
+          apply (call_api_func)
+          apply (if_block)
+          apply (call_api_func)
+          apply (if_block)
+          apply (call_api_func)
+          apply (if_block)
+          apply (call_api_func)
+          done
+      next
+        assume ?D
+        then obtain t xs tl tr encode where
+           1: "coupons = t # xs 
+         \<and> is_force_coupon t
+         \<and> get_coupon_lhs t = Some tl
+         \<and> get_coupon_rhs t = Some tr
+         \<and> create_strict_encode_api tl = Some encode"
+         and 2: "(get_type tr = 0 \<or> get_type tr = 1) \<longrightarrow> (\<not> is_equal encode l \<or> \<not> is_equal tr r)"
+          by blast
+      
+        show ?thesis
+        proof (cases "get_type tr = 0 \<or> get_type tr = 1")
+          case False
+          then have "host_func_apply_impl ?state type_r_i32 fixpoint_is_object
+  [(V_ref (ConstRefExtern (to_externref tr)))] 
+  = Some (?state, [V_num (ConstInt32 (wasm_bool False))])"
+          using fixpoint_is_object_impl[of ?state]
+          using to_handle_to_externref by presburger
+
+          then show ?thesis
+            using 1 
+                  fixpoint_is_force_coupon_impl[of ?state]
+                  fixpoint_get_coupon_lhs_impl[of ?state]
+                  fixpoint_get_coupon_rhs_impl[of ?state]
+                  fixpoint_is_equal_impl[of ?state]
+                  fixpoint_create_eq_coupon_impl[of ?state]
+                  fixpoint_create_strict_encode_impl[of ?state]
+            apply (invoke_coupon_func fuel_idx_def: plus_43 func_make_force_to_encode_strict_coupon_idx_def)
+            apply (table_get_local_set)
+            apply (call_api_func)
+            apply (if_block)
+            apply (call_api_func)
+            apply (if_block)
+            done
+        next
+          case True
+          then have 3: "host_func_apply_impl ?state type_r_i32 fixpoint_is_object
+  [(V_ref (ConstRefExtern (to_externref tr)))] 
+  = Some (?state, [V_num (ConstInt32 (wasm_bool True))])"
+            using fixpoint_is_object_impl[of ?state]
+            using to_handle_to_externref by presburger
+
+          moreover have 4: "(\<not> is_equal encode l \<or> \<not> is_equal tr r)"
+            using 2 True
+            by blast
+
+          ultimately show ?thesis
+            using 1 
+                  fixpoint_is_force_coupon_impl[of ?state]
+                  fixpoint_get_coupon_lhs_impl[of ?state]
+                  fixpoint_get_coupon_rhs_impl[of ?state]
+                  fixpoint_is_equal_impl[of ?state]
+                  fixpoint_is_object_impl[of ?state]
+                  fixpoint_create_eq_coupon_impl[of ?state]
+                  fixpoint_create_strict_encode_impl[of ?state]
+            apply (invoke_coupon_func fuel_idx_def: plus_43 func_make_force_to_encode_strict_coupon_idx_def)
+            apply (table_get_local_set)
+            apply (call_api_func)
+            apply (if_block)
+            apply (call_api_func)
+            apply (if_block)
+            apply (call_api_func)
+            apply (if_block)
+            apply (call_api_func)
+            apply (if_block)
+            done
+        qed
+      qed
+    qed
+  qed
+qed
+
+end
