wasm-proofs/Wasm-Proof/sym_coupon.thy
@@ -3,25 +3,26 @@ theory sym_coupon
 begin
 
 lemma make_some:
-  assumes "make_sym_coupon_raw coupons l r = Some res"
+  assumes "make_sym_coupon coupons l r = Some res"
   shows "\<exists>e xs l' r'.
          coupons = (e # xs)
-      \<and>  is_eq_coupon_api e
+      \<and>  is_eq_coupon e
       \<and>  get_coupon_lhs e = Some l'
       \<and>  get_coupon_rhs e = Some r'
       \<and>  is_equal r' l
       \<and>  is_equal l' r
-      \<and>  res = create_eq_coupon l r"
+      \<and>  res = create_coupon Eq l r"
 proof -
   obtain e xs l' r' where
     1: "coupons = (e # xs)
-      \<and>  is_eq_coupon_api e
+      \<and>  is_eq_coupon e
       \<and>  get_coupon_lhs e = Some l'
       \<and>  get_coupon_rhs e = Some r'"
-    by (metis assms is_coupon_lhs is_coupon_rhs is_eq_coupon_api_def make_sym_coupon_raw.elims option.simps(3))
+    by (metis assms eq_lhs_exist eq_rhs_exist if_Some_None_eq_None
+        make_sym_coupon.elims)
 
-  then have "make_sym_coupon_raw coupons l r =
-        (if (is_equal r' l \<and> is_equal l' r) then Some (create_eq_coupon l r) else None)"
+  then have "make_sym_coupon coupons l r =
+        (if (is_equal r' l \<and> is_equal l' r) then Some (create_coupon Eq l r) else None)"
     by simp
 
   then show ?thesis 
@@ -31,21 +32,21 @@ qed
 lemma make_some_rev:
   assumes "\<exists>e xs l' r'.
          coupons = (e # xs)
-      \<and>  is_eq_coupon_api e
+      \<and>  is_eq_coupon e
       \<and>  get_coupon_lhs e = Some l'
       \<and>  get_coupon_rhs e = Some r'
       \<and>  is_equal r' l
       \<and>  is_equal l' r"
-  shows "make_sym_coupon_raw coupons l r = Some (create_eq_coupon l r)"
+  shows "make_sym_coupon coupons l r = Some (create_coupon Eq l r)"
   using assms by fastforce
 
 lemma make_none:
-  assumes "make_sym_coupon_raw coupons l r = None"
+  assumes "make_sym_coupon coupons l r = None"
   shows "coupons = [] \<or>
         (\<exists>e xs. coupons = e # xs \<and>
-          (\<not>is_eq_coupon_api e \<or>
+          (\<not>is_eq_coupon e \<or>
            (\<exists>l' r'.
-            is_eq_coupon_api e \<and>
+            is_eq_coupon e \<and>
             get_coupon_lhs e = Some l' \<and>
             get_coupon_rhs e = Some r' \<and>
             (\<not>is_equal r' l \<or> \<not>is_equal l' r))))"
@@ -56,13 +57,13 @@ next
   then obtain e xs where 1: "coupons = e # xs"
     by (meson list.exhaust)
   then show ?thesis
-  proof (cases "is_eq_coupon_api e")
+  proof (cases "is_eq_coupon e")
     case False
     then show ?thesis using 1 by auto
   next
     case True
     then obtain l' r' where "get_coupon_lhs e = Some l' \<and> get_coupon_rhs e = Some r'"
-      by (meson is_coupon_lhs is_coupon_rhs is_eq_coupon_api_def)
+      using eq_lhs_exist eq_rhs_exist by blast
     then show ?thesis
       using "1" assms by force
   qed
@@ -73,8 +74,8 @@ lemma plus_33:
 (Suc (Suc (Suc (Suc (Suc (Suc (Suc(Suc (Suc (Suc (Suc (Suc (Suc (Suc (Suc (Suc (Suc (Suc (Suc (Suc (Suc (Suc (Suc (Suc (Suc (Suc (Suc (Suc (Suc (Suc n)))))))))))))))))))))))))))))))))"
   by auto
 
-lemma make_sym_coupon_raw_run_iter:
-  assumes "make_sym_coupon_raw coupons l r = Some res"
+lemma make_sym_coupon_run_iter:
+  assumes "make_sym_coupon coupons l r = Some res"
   shows "run_iter (n + 33)
           (Config 
            (Suc n')
@@ -91,16 +92,16 @@ lemma make_sym_coupon_raw_run_iter:
           (Config 
            (Suc n')
            (init\<lparr> tabs := (tabs init)[tab_coupons_idx := ((T_tab \<lparr> l_min = 0, l_max = None\<rparr> T_ext_ref), (map (\<lambda>c. (ConstRefExtern (to_externref c))) coupons))] \<rparr>)
-            (Frame_context (Redex (V_ref (ConstRefExtern (to_externref (create_eq_coupon l r))) # rest_vs) [] b_es) lc f  \<lparr>f_locs = locs, f_inst = exp_inst\<rparr>) fcs)"
+            (Frame_context (Redex (V_ref (ConstRefExtern (to_externref res)) # rest_vs) [] b_es) lc f  \<lparr>f_locs = locs, f_inst = exp_inst\<rparr>) fcs)"
 proof -
   obtain e xs l' r' where
        1: "coupons = (e # xs)
-      \<and>  is_eq_coupon_api e
+      \<and>  is_eq_coupon e
       \<and>  get_coupon_lhs e = Some l'
       \<and>  get_coupon_rhs e = Some r'
       \<and>  is_equal r' l
       \<and>  is_equal l' r
-      \<and>  res = create_eq_coupon l r"
+      \<and>  res = create_coupon Eq l r"
     using make_some[OF assms] by auto
 
     let ?state = " (init\<lparr> tabs := (tabs init)[tab_coupons_idx := ((T_tab \<lparr> l_min = 0, l_max = None\<rparr> T_ext_ref), (map (\<lambda>c. (ConstRefExtern (to_externref c))) coupons))] \<rparr> )"
@@ -124,8 +125,8 @@ proof -
       done
 qed
 
-lemma make_sym_coupon_raw_run_invoke_none:
-  assumes "make_sym_coupon_raw coupons l r = None"
+lemma make_sym_coupon_run_invoke_none:
+  assumes "make_sym_coupon coupons l r = None"
   shows "\<exists>msg cfg.
           run_iter (n + 33)
           (Config 
