wasm-proofs/Wasm-Proof/think_application_coupon.thy
@@ -1,0 +1,304 @@
+theory think_application_coupon
+  imports custom_method isabelle_coupon
+begin
+
+lemma make_some:
+  assumes "make_think_application_coupon coupons l r = Some res"
+  shows "\<exists>c1 c2 xs c1l c1r.
+         coupons = c1 # c2 # xs
+       \<and> is_eval_coupon c1
+       \<and> is_apply_coupon c2
+       \<and> get_coupon_lhs c1 = Some c1l
+       \<and> get_coupon_rhs c1 = Some c1r
+       \<and> get_coupon_lhs c2 = Some c1r
+       \<and> get_coupon_rhs c2 = Some r
+       \<and> create_application_thunk_api c1l = Some l
+       \<and> res = create_coupon Think l r"
+proof - 
+  obtain c1 c2 xs where
+       1: "coupons = c1 # c2 # xs \<and> is_eval_coupon c1 \<and> is_apply_coupon c2"
+    using assms
+    apply (cases coupons; simp_all; case_tac list; simp_all)
+    by (meson option.distinct(1))
+
+  then obtain c1l c1r c2l c2r where 2: "get_coupon_lhs c1 = Some c1l
+        \<and> get_coupon_rhs c1 = Some c1r
+        \<and> get_coupon_lhs c2 = Some c2l
+        \<and> get_coupon_rhs c2 = Some c2r"
+    using eval_lhs_exist eval_rhs_exist apply_lhs_exist apply_rhs_exist
+    by presburger
+
+  then show ?thesis
+    using 1 2 assms
+    apply simp
+    apply (cases "c1r = c2l"; simp_all)
+    apply (cases "create_application_thunk_api c1l"; simp_all)
+    by (simp add: handy_if_lemma)
+qed
+
+lemma make_some_rev:
+  assumes "\<exists>c1 c2 xs c1l c1r.
+         coupons = c1 # c2 # xs
+       \<and> is_eval_coupon c1
+       \<and> is_apply_coupon c2
+       \<and> get_coupon_lhs c1 = Some c1l
+       \<and> get_coupon_rhs c1 = Some c1r
+       \<and> get_coupon_lhs c2 = Some c1r
+       \<and> get_coupon_rhs c2 = Some r
+       \<and> create_application_thunk_api c1l = Some l"
+  shows "make_think_application_coupon coupons l r = Some (create_coupon Think l r)"
+  using assms by fastforce
+
+lemma make_none:
+  assumes "make_think_application_coupon coupons l r = None"
+  shows "(length coupons < 2) \<or>
+         (\<exists>c1 c2 xs. coupons = c1 # c2 # xs \<and>
+          (\<not>is_eval_coupon c1 \<or> \<not>is_apply_coupon c2)) \<or>
+         (\<exists>c1 c2 xs c1l c1r c2l c2r.
+          coupons = c1 # c2 # xs
+        \<and> is_eval_coupon c1
+        \<and> is_apply_coupon c2
+        \<and> get_coupon_lhs c1 = Some c1l
+        \<and> get_coupon_rhs c1 = Some c1r
+        \<and> get_coupon_lhs c2 = Some c2l
+        \<and> get_coupon_rhs c2 = Some c2r
+        \<and> (create_application_thunk_api c1l = None \<or>
+           (\<exists>thunk. create_application_thunk_api c1l = Some thunk
+             \<and> (\<not>is_equal c1r c2l 
+             \<or> \<not>is_equal thunk l 
+             \<or> \<not>is_equal c2r r)))
+       )"
+proof (cases "length coupons < 2")
+  case True then show ?thesis by auto
+next
+  case False
+  then obtain c1 c2 xs where 1 : "coupons = c1 # c2 # xs"
+    using list_length_2 by blast
+  then show ?thesis
+  proof (cases "(\<not>is_eval_coupon c1 \<or> \<not>is_apply_coupon c2)")
+    case True then show ?thesis using 1 by blast
+  next
+    case False
+    then obtain c1l c1r c2l c2r where
+         "get_coupon_lhs c1 = Some c1l
+        \<and> get_coupon_rhs c1 = Some c1r
+        \<and> get_coupon_lhs c2 = Some c2l
+        \<and> get_coupon_rhs c2 = Some c2r"
+      using eval_lhs_exist eval_rhs_exist apply_lhs_exist apply_rhs_exist
+      by presburger
+
+    then show ?thesis
+      using 1 assms
+      by fastforce
+  qed
+qed
+
+lemma plus_54:
+"n + 54 = (Suc (Suc (Suc (Suc (Suc (Suc (Suc (Suc (Suc (Suc (Suc (Suc (Suc (Suc (Suc (Suc (Suc (Suc (Suc (Suc (Suc (Suc (Suc (Suc 
+(Suc (Suc (Suc (Suc (Suc (Suc (Suc(Suc (Suc (Suc (Suc (Suc (Suc (Suc (Suc (Suc (Suc (Suc (Suc (Suc (Suc (Suc (Suc (Suc (Suc (Suc (Suc (Suc (Suc (Suc n))))))))))))))))))))))))))))))))))))))))))))))))))))))"
+  by auto
+
+lemma make_think_application_coupon_run_iter:
+  assumes "make_think_application_coupon coupons l r = Some res"
+  shows  "run_iter (n + 54)
+          (Config 
+           (Suc n')
+           (init\<lparr> tabs := (tabs init)[tab_coupons_idx := ((T_tab \<lparr> l_min = 0, l_max = None\<rparr> T_ext_ref), (map (\<lambda>c. (ConstRefExtern (to_externref c))) coupons))] \<rparr>)
+           (Frame_context 
+              (Redex ((V_ref (ConstRefExtern (to_externref r))) #
+                      (V_ref (ConstRefExtern (to_externref l))) #
+                      rest_vs)
+                     [Invoke func_make_think_application_coupon_idx]
+                     b_es)
+            lc f \<lparr>f_locs = locs, f_inst = exp_inst\<rparr>) fcs)
+ =
+          run_iter n
+          (Config 
+           (Suc n')
+           (init\<lparr> tabs := (tabs init)[tab_coupons_idx := ((T_tab \<lparr> l_min = 0, l_max = None\<rparr> T_ext_ref), (map (\<lambda>c. (ConstRefExtern (to_externref c))) coupons))] \<rparr>)
+            (Frame_context (Redex (V_ref (ConstRefExtern (to_externref res)) # rest_vs) [] b_es) lc f  \<lparr>f_locs = locs, f_inst = exp_inst\<rparr>) fcs)"
+proof -
+  obtain c1 c2 xs c1l c1r where
+         1: "coupons = c1 # c2 # xs
+       \<and> is_eval_coupon c1
+       \<and> is_apply_coupon c2
+       \<and> get_coupon_lhs c1 = Some c1l
+       \<and> get_coupon_rhs c1 = Some c1r
+       \<and> get_coupon_lhs c2 = Some c1r
+       \<and> get_coupon_rhs c2 = Some r
+       \<and> create_application_thunk_api c1l = Some l
+       \<and> res = create_coupon Think l r"
+    using make_some[OF assms] by auto
+
+  let ?state = " (init\<lparr> tabs := (tabs init)[tab_coupons_idx := ((T_tab \<lparr> l_min = 0, l_max = None\<rparr> T_ext_ref), (map (\<lambda>c. (ConstRefExtern (to_externref c))) coupons))] \<rparr> )"
+
+  show ?thesis
+    using 1 
+          fixpoint_is_eval_coupon_impl[of ?state]
+          fixpoint_is_apply_coupon_impl[of ?state]
+          fixpoint_get_coupon_lhs_impl[of ?state]
+          fixpoint_get_coupon_rhs_impl[of ?state]
+          fixpoint_is_equal_impl[of ?state]
+          fixpoint_create_think_coupon_impl[of ?state]
+          fixpoint_create_application_thunk_impl[of ?state]
+    apply (invoke_coupon_func fuel_idx_def: plus_54 func_make_think_application_coupon_idx_def)
+     apply (table_get_local_set)
+     apply (call_api_func)
+     apply (if_block)
+     apply (call_api_func)
+     apply (if_block)
+     apply (call_api_func)
+     apply (if_block)
+     apply (call_api_func)
+     apply (if_block)
+     apply (call_api_func)
+     apply (if_block)
+     apply (call_api_func)
+     done
+qed
+
+lemma make_think_application_coupon_run_invoke_none:
+  assumes "make_think_application_coupon coupons l r = None"
+  shows "\<exists>msg cfg.
+         run_iter (n + 54)
+          (Config 
+           (Suc n')
+           (init\<lparr> tabs := (tabs init)[tab_coupons_idx := ((T_tab \<lparr> l_min = 0, l_max = None\<rparr> T_ext_ref), (map (\<lambda>c. (ConstRefExtern (to_externref c))) coupons))] \<rparr>)
+           (Frame_context 
+              (Redex ((V_ref (ConstRefExtern (to_externref r))) #
+                      (V_ref (ConstRefExtern (to_externref l))) #
+                      rest_vs)
+                     [Invoke func_make_think_application_coupon_idx]
+                     b_es)
+            lc f \<lparr>f_locs = locs, f_inst = exp_inst\<rparr>) fcs)
+ = (cfg, RTrap msg)"
+proof -
+  let ?A = "length coupons < 2"
+  let ?B = "\<exists>c1 c2 xs. coupons = c1 # c2 # xs \<and>
+          (\<not>is_eval_coupon c1 \<or> \<not>is_apply_coupon c2)"
+  let ?C = "(\<exists>c1 c2 xs c1l c1r c2l c2r.
+          coupons = c1 # c2 # xs
+        \<and> is_eval_coupon c1
+        \<and> is_apply_coupon c2
+        \<and> get_coupon_lhs c1 = Some c1l
+        \<and> get_coupon_rhs c1 = Some c1r
+        \<and> get_coupon_lhs c2 = Some c2l
+        \<and> get_coupon_rhs c2 = Some c2r
+        \<and> (create_application_thunk_api c1l = None \<or>
+           (\<exists>thunk. create_application_thunk_api c1l = Some thunk
+             \<and> (\<not>is_equal c1r c2l 
+             \<or> \<not>is_equal thunk l 
+             \<or> \<not>is_equal c2r r)))
+       )"
+
+  let ?state = "(init\<lparr> tabs := (tabs init)[tab_coupons_idx := ((T_tab \<lparr> l_min = 0, l_max = None\<rparr> T_ext_ref), (map (\<lambda>c. (ConstRefExtern (to_externref c))) coupons))] \<rparr>)"
+
+
+  have assms: "?A \<or> ?B \<or> ?C" 
+    using make_none[OF assms] by blast
+
+  show ?thesis
+    using assms
+  proof
+    assume "?A"
+    then have "\<not> nat_of_int (I32.lift0 1) < length coupons"
+      by (simp add: nat_of_int_i32.abs_eq)
+    then show ?thesis
+      apply (invoke_coupon_func fuel_idx_def: plus_54 func_make_think_application_coupon_idx_def)
+      apply (table_get_local_set)
+      done
+  next
+    assume "?B \<or> ?C"
+    then show ?thesis
+    proof
+      assume "?B"
+      then obtain c1 c2 xs where
+        "coupons = c1 # c2 # xs"
+        and "\<not> is_eval_coupon c1 \<or> (is_eval_coupon c1 \<and> \<not> is_apply_coupon c2)"
+        by blast
+      then show ?thesis
+        using fixpoint_is_eval_coupon_impl[of ?state]
+        fixpoint_is_apply_coupon_impl[of ?state]
+        apply (invoke_coupon_func fuel_idx_def: plus_54 func_make_think_application_coupon_idx_def)
+        apply (table_get_local_set)
+        apply (call_api_func)
+        apply (if_block)
+        apply (call_api_func)
+        apply (if_block)
+        done
+    next
+      assume "?C"
+      then obtain c1 c2 xs c1l c1r c2l c2r where
+        1: "coupons = c1 # c2 # xs \<and>
+         is_eval_coupon c1 \<and>
+         is_apply_coupon c2 \<and>
+         get_coupon_lhs c1 = Some c1l \<and>
+         get_coupon_rhs c1 = Some c1r \<and>
+         get_coupon_lhs c2 = Some c2l \<and>
+         get_coupon_rhs c2 = Some c2r"
+      and  2: "(create_application_thunk_api c1l = None \<or>
+      (\<exists>thunk.
+          create_application_thunk_api c1l = Some thunk \<and>
+          (\<not> is_equal c1r c2l \<or> \<not> is_equal thunk l \<or> \<not> is_equal c2r r)))"
+        by blast
+
+      show ?thesis
+        using 2
+      proof
+        assume "create_application_thunk_api c1l = None"
+        then show ?thesis
+          using 1
+            fixpoint_is_eval_coupon_impl[of ?state]
+            fixpoint_is_apply_coupon_impl[of ?state]
+            fixpoint_get_coupon_lhs_impl[of ?state]
+            fixpoint_get_coupon_rhs_impl[of ?state]
+            fixpoint_is_equal_impl[of ?state]
+            fixpoint_create_think_coupon_impl[of ?state]
+            fixpoint_create_application_thunk_impl[of ?state]
+          apply (invoke_coupon_func fuel_idx_def: plus_54 func_make_think_application_coupon_idx_def)
+          apply (table_get_local_set)
+          apply (call_api_func)
+          apply (if_block)
+          apply (call_api_func)
+          apply (if_block)
+          apply (call_api_func)
+          apply (if_block)
+          apply (call_api_func)
+          done
+      next
+        assume "(\<exists>thunk.
+          create_application_thunk_api c1l = Some thunk \<and>
+          (\<not> is_equal c1r c2l \<or> \<not> is_equal thunk l \<or> \<not> is_equal c2r r))"
+        then obtain thunk 
+          where "create_application_thunk_api c1l = Some thunk" 
+            and "(\<not> is_equal c1r c2l \<or> \<not> is_equal thunk l \<or> \<not> is_equal c2r r)" 
+          by blast
+
+        then show ?thesis
+          using 1
+            fixpoint_is_eval_coupon_impl[of ?state]
+            fixpoint_is_apply_coupon_impl[of ?state]
+            fixpoint_get_coupon_lhs_impl[of ?state]
+            fixpoint_get_coupon_rhs_impl[of ?state]
+            fixpoint_is_equal_impl[of ?state]
+            fixpoint_create_think_coupon_impl[of ?state]
+            fixpoint_create_application_thunk_impl[of ?state]
+          apply (invoke_coupon_func fuel_idx_def: plus_54 func_make_think_application_coupon_idx_def)
+          apply (table_get_local_set)
+          apply (call_api_func)
+          apply (if_block)
+          apply (call_api_func)
+          apply (if_block)
+          apply (call_api_func)
+          apply (if_block)
+          apply (call_api_func)
+          apply (if_block)
+          apply (call_api_func)
+          apply (if_block)
+          done
+      qed
+    qed
+  qed
+qed
+
+end
