wasm-proofs/Wasm-Proof/think_to_force_coupon.thy
@@ -1,0 +1,247 @@
+theory think_to_force_coupon
+  imports custom_method isabelle_coupon
+begin
+
+lemma make_some:
+  assumes "make_think_to_force_coupon coupons l r = Some res"
+  shows "\<exists>t xs.
+         coupons = t # xs
+       \<and> is_think_coupon t
+       \<and> get_coupon_lhs t = Some l
+       \<and> get_coupon_rhs t = Some r
+       \<and> (get_type r = 0 \<or> get_type r = 1 \<or> get_type r = 2 \<or> get_type r = 3)
+       \<and> res = create_coupon Force l r"
+proof -
+  obtain t xs where 1: "coupons = t # xs \<and> is_think_coupon t"
+    using assms
+    apply (cases coupons; simp_all)
+    by fastforce
+
+  then obtain tl tr where 2: "get_coupon_lhs t = Some tl \<and> get_coupon_rhs t = Some tr"
+    using think_lhs_exist think_rhs_exist
+    by presburger
+
+  show ?thesis
+    using 1 2 assms
+    by (simp, metis is_equal_match option.distinct(1) option.sel)
+qed
+
+lemma make_none:
+  assumes "make_think_to_force_coupon coupons l r = None" 
+  shows "(length coupons = 0) \<or>
+         (\<exists>t xs. coupons = t # xs \<and> \<not> is_think_coupon t) \<or>
+         (\<exists>t xs tl tr. 
+           coupons = t # xs 
+         \<and> is_think_coupon t
+         \<and> get_coupon_lhs t = Some tl
+         \<and> get_coupon_rhs t = Some tr
+         \<and> ((get_type tr = 0 \<or> get_type tr = 1 \<or> get_type tr = 2 \<or> get_type tr = 3) \<longrightarrow> (\<not> is_equal tl l \<or> \<not> is_equal tr r)))"
+proof (cases "length coupons = 0")
+  case True then show ?thesis by auto
+next
+  case False
+  then obtain t xs where 1: "coupons = t # xs"
+    by (metis list.exhaust list.size(3))
+  then show ?thesis
+  proof (cases "is_think_coupon t")
+    case False then show ?thesis
+      using 1 by blast
+  next
+    case True
+    then obtain tl tr where
+         "get_coupon_lhs t = Some tl
+        \<and> get_coupon_rhs t = Some tr"
+      using think_lhs_exist think_rhs_exist
+      by presburger
+
+    then show ?thesis
+      using 1 assms
+      by fastforce
+  qed
+qed
+
+lemma plus_41:
+"n + 41 = (Suc (Suc (Suc (Suc (Suc (Suc (Suc (Suc (Suc (Suc (Suc 
+(Suc (Suc (Suc (Suc (Suc (Suc (Suc(Suc (Suc (Suc (Suc (Suc (Suc (Suc (Suc (Suc (Suc (Suc (Suc (Suc (Suc (Suc (Suc (Suc (Suc (Suc (Suc (Suc (Suc (Suc n)))))))))))))))))))))))))))))))))))))))))"
+  by auto
+
+lemma make_think_to_force_coupon_run_iter:
+  assumes "make_think_to_force_coupon coupons l r = Some res"
+  shows  "run_iter (n + 41)
+          (Config 
+           (Suc n')
+           (init\<lparr> tabs := (tabs init)[tab_coupons_idx := ((T_tab \<lparr> l_min = 0, l_max = None\<rparr> T_ext_ref), (map (\<lambda>c. (ConstRefExtern (to_externref c))) coupons))] \<rparr>)
+           (Frame_context 
+              (Redex ((V_ref (ConstRefExtern (to_externref r))) #
+                      (V_ref (ConstRefExtern (to_externref l))) #
+                      rest_vs)
+                     [Invoke func_make_think_to_force_coupon_idx]
+                     b_es)
+            lc f \<lparr>f_locs = locs, f_inst = exp_inst\<rparr>) fcs)
+ =
+          run_iter n
+          (Config 
+           (Suc n')
+           (init\<lparr> tabs := (tabs init)[tab_coupons_idx := ((T_tab \<lparr> l_min = 0, l_max = None\<rparr> T_ext_ref), (map (\<lambda>c. (ConstRefExtern (to_externref c))) coupons))] \<rparr>)
+            (Frame_context (Redex (V_ref (ConstRefExtern (to_externref res)) # rest_vs) [] b_es) lc f  \<lparr>f_locs = locs, f_inst = exp_inst\<rparr>) fcs)"
+proof -
+  obtain t xs where
+         1: "coupons = t # xs
+       \<and> is_think_coupon t
+       \<and> get_coupon_lhs t = Some l
+       \<and> get_coupon_rhs t = Some r
+       \<and> (get_type r = 0 \<or> get_type r = 1 \<or> get_type r = 2 \<or> get_type r = 3)
+       \<and> res = create_coupon Force l r"
+    using make_some[OF assms] by auto
+
+  let ?state = " (init\<lparr> tabs := (tabs init)[tab_coupons_idx := ((T_tab \<lparr> l_min = 0, l_max = None\<rparr> T_ext_ref), (map (\<lambda>c. (ConstRefExtern (to_externref c))) coupons))] \<rparr> )"
+
+  show ?thesis
+    using 1 
+          fixpoint_is_think_coupon_impl[of ?state]
+          fixpoint_get_coupon_lhs_impl[of ?state]
+          fixpoint_get_coupon_rhs_impl[of ?state]
+          fixpoint_is_equal_impl[of ?state]
+          fixpoint_is_data_impl[of ?state]
+          fixpoint_create_force_coupon_impl[of ?state]
+    apply (invoke_coupon_func fuel_idx_def: plus_41 func_make_think_to_force_coupon_idx_def)
+    apply (table_get_local_set)
+    apply (call_api_func)
+    apply (if_block)
+    apply (call_api_func)
+    apply (if_block)
+    apply (call_api_func)
+    apply (if_block)
+    apply (call_api_func)
+    apply (if_block)
+    apply (call_api_func)
+    done
+qed
+
+lemma make_think_to_force_coupon_run_invoke_none:
+  assumes "make_think_to_force_coupon coupons l r = None"
+  shows "\<exists>msg cfg.
+         run_iter (n + 41)
+          (Config 
+           (Suc n')
+           (init\<lparr> tabs := (tabs init)[tab_coupons_idx := ((T_tab \<lparr> l_min = 0, l_max = None\<rparr> T_ext_ref), (map (\<lambda>c. (ConstRefExtern (to_externref c))) coupons))] \<rparr>)
+           (Frame_context 
+              (Redex ((V_ref (ConstRefExtern (to_externref r))) #
+                      (V_ref (ConstRefExtern (to_externref l))) #
+                      rest_vs)
+                     [Invoke func_make_think_to_force_coupon_idx]
+                     b_es)
+            lc f \<lparr>f_locs = locs, f_inst = exp_inst\<rparr>) fcs)
+ = (cfg, RTrap msg)"
+proof -
+  let ?A = "length coupons = 0"
+  let ?B = "\<exists>t xs. coupons = t # xs \<and> \<not> is_think_coupon t"
+  let ?C = "\<exists>t xs tl tr. 
+           coupons = t # xs 
+         \<and> is_think_coupon t
+         \<and> get_coupon_lhs t = Some tl
+         \<and> get_coupon_rhs t = Some tr
+         \<and> ((get_type tr = 0 \<or> get_type tr = 1 \<or> get_type tr = 2 \<or> get_type tr = 3) \<longrightarrow> (\<not> is_equal tl l \<or> \<not> is_equal tr r))"
+
+  let ?state = "(init\<lparr> tabs := (tabs init)[tab_coupons_idx := ((T_tab \<lparr> l_min = 0, l_max = None\<rparr> T_ext_ref), (map (\<lambda>c. (ConstRefExtern (to_externref c))) coupons))] \<rparr>)"
+
+  have assms: "?A \<or> ?B \<or> ?C" 
+    using make_none[OF assms] by blast
+
+  show ?thesis
+    using assms
+  proof
+    assume ?A
+    then have "\<not> nat_of_int (I32.lift0 0) < length coupons"
+      by (simp add: nat_of_int_i32.abs_eq)
+    then show ?thesis
+      apply (invoke_coupon_func fuel_idx_def: plus_41 func_make_think_to_force_coupon_idx_def)
+      apply (table_get_local_set)
+      done
+  next
+    assume "?B \<or> ?C"
+    then show ?thesis
+    proof
+      assume ?B
+      then obtain t xs where
+        "coupons = t # xs"
+     and "\<not>is_think_coupon t" by blast
+
+      then show ?thesis
+        using fixpoint_is_think_coupon_impl[of ?state]
+        apply (invoke_coupon_func fuel_idx_def: plus_41 func_make_think_to_force_coupon_idx_def)
+        apply (table_get_local_set)
+        apply (call_api_func)
+        apply (if_block)
+        done
+    next
+      assume ?C
+      then obtain t xs tl tr where
+        1: "coupons = t # xs \<and>
+        is_think_coupon t \<and>
+        get_coupon_lhs t = Some tl \<and>
+        get_coupon_rhs t = Some tr"
+        and 2: "(get_type tr = 0 \<or> get_type tr = 1 \<or> get_type tr = 2 \<or> get_type tr = 3 \<longrightarrow>
+         \<not> is_equal tl l \<or> \<not> is_equal tr r) "
+        by blast
+
+      show ?thesis
+      proof (cases "get_type tr = 0 \<or> get_type tr = 1 \<or> get_type tr = 2 \<or> get_type tr = 3")
+        case False
+        then have "host_func_apply_impl ?state type_r_i32 fixpoint_is_data
+  [(V_ref (ConstRefExtern (to_externref tr)))] 
+  = Some (?state, [V_num (ConstInt32 (wasm_bool False))])"
+          using fixpoint_is_data_impl[of ?state]
+          using to_handle_to_externref by presburger
+        
+        then show ?thesis
+          using 1
+            fixpoint_is_think_coupon_impl[of ?state]
+            fixpoint_get_coupon_lhs_impl[of ?state]
+            fixpoint_get_coupon_rhs_impl[of ?state]
+            fixpoint_is_equal_impl[of ?state]
+            fixpoint_create_force_coupon_impl[of ?state]
+          apply (invoke_coupon_func fuel_idx_def: plus_41 func_make_think_to_force_coupon_idx_def)
+          apply (table_get_local_set)
+          apply (call_api_func)
+          apply (if_block)
+          apply (call_api_func)
+          apply (if_block)
+          done
+      next
+        case True
+        then have 3: "host_func_apply_impl ?state type_r_i32 fixpoint_is_data
+  [(V_ref (ConstRefExtern (to_externref tr)))] 
+  = Some (?state, [V_num (ConstInt32 (wasm_bool True))])"
+          using fixpoint_is_data_impl[of ?state]
+          using to_handle_to_externref by presburger
+
+        moreover have 4: "(\<not> is_equal tl l \<or> \<not> is_equal tr r)"
+          using 2 True
+          by blast
+
+        ultimately show ?thesis
+          using 1 
+            fixpoint_is_think_coupon_impl[of ?state]
+            fixpoint_get_coupon_lhs_impl[of ?state]
+            fixpoint_get_coupon_rhs_impl[of ?state]
+            fixpoint_is_equal_impl[of ?state]
+            fixpoint_is_data_impl[of ?state]
+            fixpoint_create_force_coupon_impl[of ?state]
+          apply (invoke_coupon_func fuel_idx_def: plus_41 func_make_think_to_force_coupon_idx_def)
+          apply (table_get_local_set)
+          apply (call_api_func)
+          apply (if_block)
+          apply (call_api_func)
+          apply (if_block)
+          apply (call_api_func)
+          apply (if_block)
+          apply (call_api_func)
+          apply (if_block)
+          done
+      qed
+    qed
+  qed
+qed
+
+end
